added binary DCA intersection, adjusted naming scheme

thys/Transition_Systems_and_Automata/Automata/DBA_Combine.thy
@@ -4,39 +4,39 @@ theory DBA_Combine
 imports "DBA" "DGBA"
 begin
 
-  definition dbai' :: "('label, 'state) dba list \<Rightarrow> ('label, 'state list) dgba" where
-    "dbai' AA \<equiv> dgba
+  definition dbgail :: "('label, 'state) dba list \<Rightarrow> ('label, 'state list) dgba" where
+    "dbgail AA \<equiv> dgba
       (INTER (set AA) dba.alphabet)
       (map dba.initial AA)
       (\<lambda> a pp. map2 (\<lambda> A p. dba.succ A a p) AA pp)
       (map (\<lambda> k pp. dba.accepting (AA ! k) (pp ! k)) [0 ..< length AA])"
 
-  lemma dbai'_trace_smap:
+  lemma dbgail_trace_smap:
     assumes "length pp = length AA" "k < length AA"
-    shows "smap (\<lambda> pp. pp ! k) (dgba.trace (dbai' AA) w pp) = dba.trace (AA ! k) w (pp ! k)"
-    using assms unfolding dbai'_def by (coinduction arbitrary: w pp) (force)
+    shows "smap (\<lambda> pp. pp ! k) (dgba.trace (dbgail AA) w pp) = dba.trace (AA ! k) w (pp ! k)"
+    using assms unfolding dbgail_def by (coinduction arbitrary: w pp) (force)
 
-  lemma dbai'_language: "DGBA.language (dbai' AA) = INTER (set AA) DBA.language"
+  lemma dbgail_language: "DGBA.language (dbgail AA) = INTER (set AA) DBA.language"
   proof safe
     fix w A
-    assume 1: "w \<in> DGBA.language (dbai' AA)" "A \<in> set AA"
+    assume 1: "w \<in> DGBA.language (dbgail AA)" "A \<in> set AA"
     obtain 2:
-      "dgba.run (dbai' AA) w (dgba.initial (dbai' AA))"
-      "gen infs (dgba.accepting (dbai' AA)) (dgba.trace (dbai' AA) w (dgba.initial (dbai' AA)))"
+      "dgba.run (dbgail AA) w (dgba.initial (dbgail AA))"
+      "gen infs (dgba.accepting (dbgail AA)) (dgba.trace (dbgail AA) w (dgba.initial (dbgail AA)))"
       using 1(1) by rule
     obtain k where 3: "A = AA ! k" "k < length AA" using 1(2) unfolding in_set_conv_nth by auto
-    have 4: "(\<lambda> pp. dba.accepting A (pp ! k)) \<in> set (dgba.accepting (dbai' AA))"
-      using 3 unfolding dbai'_def by auto
+    have 4: "(\<lambda> pp. dba.accepting A (pp ! k)) \<in> set (dgba.accepting (dbgail AA))"
+      using 3 unfolding dbgail_def by auto
     show "w \<in> DBA.language A"
     proof
       show "dba.run A w (dba.initial A)"
-        using 1(2) 2(1) unfolding DBA.run_alt_def DGBA.run_alt_def dbai'_def by auto
-      have "True \<longleftrightarrow> infs (\<lambda> pp. dba.accepting A (pp ! k)) (dgba.trace (dbai' AA) w (map dba.initial AA))"
-        using 2(2) 4 unfolding dbai'_def by auto
+        using 1(2) 2(1) unfolding DBA.run_alt_def DGBA.run_alt_def dbgail_def by auto
+      have "True \<longleftrightarrow> infs (\<lambda> pp. dba.accepting A (pp ! k)) (dgba.trace (dbgail AA) w (map dba.initial AA))"
+        using 2(2) 4 unfolding dbgail_def by auto
       also have "\<dots> \<longleftrightarrow> infs (dba.accepting A) (smap (\<lambda> pp. pp ! k)
-        (dgba.trace (dbai' AA) w (map dba.initial AA)))" by (simp add: comp_def)
-      also have "smap (\<lambda> pp. pp ! k) (dgba.trace (dbai' AA) w (map dba.initial AA)) =
-        dba.trace (AA ! k) w (map dba.initial AA ! k)" using 3(2) by (fastforce intro: dbai'_trace_smap)
+        (dgba.trace (dbgail AA) w (map dba.initial AA)))" by (simp add: comp_def)
+      also have "smap (\<lambda> pp. pp ! k) (dgba.trace (dbgail AA) w (map dba.initial AA)) =
+        dba.trace (AA ! k) w (map dba.initial AA ! k)" using 3(2) by (fastforce intro: dbgail_trace_smap)
       also have "\<dots> = dba.trace A w (dba.initial A)" using 3 by auto
       finally show "infs (dba.accepting A) (dba.trace A w (dba.initial A))" by simp
     qed
@@ -45,70 +45,70 @@ begin
     assume 1: "w \<in> INTER (set AA) DBA.language"
     have 2: "dba.run A w (dba.initial A)" "infs (dba.accepting A) (dba.trace A w (dba.initial A))"
       if "A \<in> set AA" for A using 1 that by auto
-    show "w \<in> DGBA.language (dbai' AA)"
+    show "w \<in> DGBA.language (dbgail AA)"
     proof (intro DGBA.language ballI gen)
-      show "dgba.run (dbai' AA) w (dgba.initial (dbai' AA))"
-        using 2(1) unfolding DBA.run_alt_def DGBA.run_alt_def dbai'_def by auto
+      show "dgba.run (dbgail AA) w (dgba.initial (dbgail AA))"
+        using 2(1) unfolding DBA.run_alt_def DGBA.run_alt_def dbgail_def by auto
     next
       fix P
-      assume 3: "P \<in> set (dgba.accepting (dbai' AA))"
+      assume 3: "P \<in> set (dgba.accepting (dbgail AA))"
       obtain k where 4: "P = (\<lambda> pp. dba.accepting (AA ! k) (pp ! k))" "k < length AA"
-        using 3 unfolding dbai'_def by auto
+        using 3 unfolding dbgail_def by auto
       have "True \<longleftrightarrow> infs (dba.accepting (AA ! k)) (dba.trace (AA ! k) w (map dba.initial AA ! k))"
         using 2(2) 4(2) by auto
       also have "dba.trace (AA ! k) w (map dba.initial AA ! k) =
-        smap (\<lambda> pp. pp ! k) (dgba.trace (dbai' AA) w (map dba.initial AA))"
-        using 4(2) by (fastforce intro: dbai'_trace_smap[symmetric])
-      also have "infs (dba.accepting (AA ! k)) \<dots> \<longleftrightarrow> infs P (dgba.trace (dbai' AA) w (map dba.initial AA))"
+        smap (\<lambda> pp. pp ! k) (dgba.trace (dbgail AA) w (map dba.initial AA))"
+        using 4(2) by (fastforce intro: dbgail_trace_smap[symmetric])
+      also have "infs (dba.accepting (AA ! k)) \<dots> \<longleftrightarrow> infs P (dgba.trace (dbgail AA) w (map dba.initial AA))"
         unfolding 4(1) by (simp add: comp_def)
-      also have "map dba.initial AA = dgba.initial (dbai' AA)" unfolding dbai'_def by simp
-      finally show "infs P (dgba.trace (dbai' AA) w (dgba.initial (dbai' AA)))" by simp
+      also have "map dba.initial AA = dgba.initial (dbgail AA)" unfolding dbgail_def by simp
+      finally show "infs P (dgba.trace (dbgail AA) w (dgba.initial (dbgail AA)))" by simp
     qed
   qed
 
-  definition dbai :: "('label, 'state) dba list \<Rightarrow> ('label, 'state list degen) dba" where
-    "dbai = degen \<circ> dbai'"
+  definition dbail :: "('label, 'state) dba list \<Rightarrow> ('label, 'state list degen) dba" where
+    "dbail = degen \<circ> dbgail"
 
-  lemma dbai_language: "DBA.language (dbai AA) = INTER (set AA) DBA.language"
-    unfolding dbai_def using degen_language dbai'_language by auto
+  lemma dbail_language: "DBA.language (dbail AA) = INTER (set AA) DBA.language"
+    unfolding dbail_def using degen_language dbgail_language by auto
 
-  definition dbau :: "('label, 'state) dba list \<Rightarrow> ('label, 'state list) dba" where
-    "dbau AA \<equiv> dba
+  definition dbaul :: "('label, 'state) dba list \<Rightarrow> ('label, 'state list) dba" where
+    "dbaul AA \<equiv> dba
       (UNION (set AA) dba.alphabet)
       (map dba.initial AA)
       (\<lambda> a pp. map2 (\<lambda> A p. dba.succ A a p) AA pp)
       (\<lambda> pp. \<exists> k < length AA. dba.accepting (AA ! k) (pp ! k))"
 
-  lemma dbau_trace_smap:
+  lemma dbaul_trace_smap:
     assumes "length pp = length AA" "k < length AA"
-    shows "smap (\<lambda> pp. pp ! k) (dba.trace (dbau AA) w pp) = dba.trace (AA ! k) w (pp ! k)"
-    using assms unfolding dbau_def by (coinduction arbitrary: w pp) (force)
+    shows "smap (\<lambda> pp. pp ! k) (dba.trace (dbaul AA) w pp) = dba.trace (AA ! k) w (pp ! k)"
+    using assms unfolding dbaul_def by (coinduction arbitrary: w pp) (force)
 
-  lemma dbau_language:
+  lemma dbaul_language:
     assumes "INTER (set AA) dba.alphabet = UNION (set AA) dba.alphabet"
-    shows "DBA.language (dbau AA) = UNION (set AA) DBA.language"
+    shows "DBA.language (dbaul AA) = UNION (set AA) DBA.language"
   proof safe
     fix w
-    assume 1: "w \<in> DBA.language (dbau AA)"
+    assume 1: "w \<in> DBA.language (dbaul AA)"
     obtain 2:
-      "dba.run (dbau AA) w (dba.initial (dbau AA))"
-      "infs (dba.accepting (dbau AA)) (dba.trace (dbau AA) w (dba.initial (dbau AA)))"
+      "dba.run (dbaul AA) w (dba.initial (dbaul AA))"
+      "infs (dba.accepting (dbaul AA)) (dba.trace (dbaul AA) w (dba.initial (dbaul AA)))"
       using 1 by rule
     obtain k where 3:
       "k < length AA"
-      "infs (\<lambda> pp. dba.accepting (AA ! k) (pp ! k)) (dba.trace (dbau AA) w (map dba.initial AA))"
-      using 2(2) unfolding dbau_def by auto
+      "infs (\<lambda> pp. dba.accepting (AA ! k) (pp ! k)) (dba.trace (dbaul AA) w (map dba.initial AA))"
+      using 2(2) unfolding dbaul_def by auto
     show "w \<in> UNION (set AA) DBA.language"
     proof (intro UN_I DBA.language)
       show "AA ! k \<in> set AA" using 3(1) by simp
       show "dba.run (AA ! k) w (dba.initial (AA ! k))"
-        using assms 2(1) 3(1) unfolding DBA.run_alt_def DGBA.run_alt_def dbau_def by force
+        using assms 2(1) 3(1) unfolding DBA.run_alt_def DGBA.run_alt_def dbaul_def by force
       have "True \<longleftrightarrow> infs (\<lambda> pp. dba.accepting (AA ! k) (pp ! k))
-        (dba.trace (dbau AA) w (map dba.initial AA))" using 3(2) by auto
+        (dba.trace (dbaul AA) w (map dba.initial AA))" using 3(2) by auto
       also have "\<dots> \<longleftrightarrow> infs (dba.accepting (AA ! k))
-        (smap (\<lambda> pp. pp ! k) (dba.trace (dbau AA) w (map dba.initial AA)))" by (simp add: comp_def)
-      also have "smap (\<lambda> pp. pp ! k) (dba.trace (dbau AA) w (map dba.initial AA)) =
-        dba.trace (AA ! k) w (map dba.initial AA ! k)" using 3(1) by (fastforce intro: dbau_trace_smap)
+        (smap (\<lambda> pp. pp ! k) (dba.trace (dbaul AA) w (map dba.initial AA)))" by (simp add: comp_def)
+      also have "smap (\<lambda> pp. pp ! k) (dba.trace (dbaul AA) w (map dba.initial AA)) =
+        dba.trace (AA ! k) w (map dba.initial AA ! k)" using 3(1) by (fastforce intro: dbaul_trace_smap)
       also have "\<dots> = dba.trace (AA ! k) w (dba.initial (AA ! k))" using 3 by auto
       finally show "infs (dba.accepting (AA ! k)) (dba.trace (AA ! k) w (dba.initial (AA ! k)))" by simp
     qed
@@ -118,19 +118,19 @@ begin
     obtain 2: "dba.run A w (dba.initial A)" "infs (dba.accepting A) (dba.trace A w (dba.initial A))"
       using 1(2) by rule
     obtain k where 3: "A = AA ! k" "k < length AA" using 1(1) unfolding in_set_conv_nth by auto
-    show "w \<in> DBA.language (dbau AA)"
+    show "w \<in> DBA.language (dbaul AA)"
     proof
-      show "dba.run (dbau AA) w (dba.initial (dbau AA))"
-        using 1(1) 2(1) unfolding DBA.run_alt_def DGBA.run_alt_def dbau_def by auto
+      show "dba.run (dbaul AA) w (dba.initial (dbaul AA))"
+        using 1(1) 2(1) unfolding DBA.run_alt_def DGBA.run_alt_def dbaul_def by auto
       have "True \<longleftrightarrow> infs (dba.accepting (AA ! k)) (dba.trace (AA ! k) w (map dba.initial AA ! k))"
         using 2(2) 3 by auto
       also have "dba.trace (AA ! k) w (map dba.initial AA ! k) =
-        smap (\<lambda> pp. pp ! k) (dba.trace (dbau AA) w (map dba.initial AA))"
-        using 3(2) by (fastforce intro: dbau_trace_smap[symmetric])
+        smap (\<lambda> pp. pp ! k) (dba.trace (dbaul AA) w (map dba.initial AA))"
+        using 3(2) by (fastforce intro: dbaul_trace_smap[symmetric])
       also have "infs (dba.accepting (AA ! k)) \<dots> \<longleftrightarrow> infs (\<lambda> pp. dba.accepting (AA ! k) (pp ! k))
-        (dba.trace (dbau AA) w (map dba.initial AA))" by (simp add: comp_def)
-      finally show "infs (dba.accepting (dbau AA)) (dba.trace (dbau AA) w (dba.initial (dbau AA)))"
-        using 3(2) unfolding dbau_def by auto
+        (dba.trace (dbaul AA) w (map dba.initial AA))" by (simp add: comp_def)
+      finally show "infs (dba.accepting (dbaul AA)) (dba.trace (dbaul AA) w (dba.initial (dbaul AA)))"
+        using 3(2) unfolding dbaul_def by auto
     qed
   qed
 
