thys/Transition_Systems_and_Automata/Automata/DRA_Combine.thy
@@ -16,101 +16,99 @@ begin
   lemma from_dca_language: "DRA.language (from_dca A) = DCA.language A"
     unfolding DCA.language_def DRA.language_def from_dca_def DCA.run_def DRA.run_def by (auto 0 3)
 
-  definition dbcai :: "('label, 'state\<^sub>1) dba \<Rightarrow> ('label, 'state\<^sub>2) dca \<Rightarrow> ('label, 'state\<^sub>1 \<times> 'state\<^sub>2) dra" where
-    "dbcai A B \<equiv> dra
+  definition dbcrai :: "('label, 'state\<^sub>1) dba \<Rightarrow> ('label, 'state\<^sub>2) dca \<Rightarrow> ('label, 'state\<^sub>1 \<times> 'state\<^sub>2) dra" where
+    "dbcrai A B \<equiv> dra
       (dba.alphabet A \<inter> dca.alphabet B)
       (dba.initial A, dca.initial B)
       (\<lambda> a (p, q). (dba.succ A a p, dca.succ B a q))
       [(dba.accepting A \<circ> fst, dca.rejecting B \<circ> snd)]"
 
-  lemma dbcai_fst[iff]: "infs (P \<circ> fst) (dra.trace (dbcai A B) w (p, q)) \<longleftrightarrow> infs P (dba.trace A w p)"
+  lemma dbcrai_fst[iff]: "infs (P \<circ> fst) (dra.trace (dbcrai A B) w (p, q)) \<longleftrightarrow> infs P (dba.trace A w p)"
   proof -
-    have "infs (P \<circ> fst) (dra.trace (dbcai A B) w (p, q)) \<longleftrightarrow>
-      infs P (smap fst (dra.trace (dbcai A B) w (p, q)))" by simp
-    also have "smap fst (dra.trace (dbcai A B) w (p, q)) = dba.trace A w p"
-      unfolding dbcai_def by (coinduction arbitrary: w p q) (auto)
+    let ?t = "dra.trace (dbcrai A B) w (p, q)"
+    have "infs (P \<circ> fst) ?t \<longleftrightarrow> infs P (smap fst ?t)" by simp
+    also have "smap fst ?t = dba.trace A w p" unfolding dbcrai_def by (coinduction arbitrary: w p q) (auto)
     finally show ?thesis by this
   qed
-  lemma dbcai_snd[iff]: "infs (P \<circ> snd) (dra.trace (dbcai A B) w (p, q)) \<longleftrightarrow> infs P (dca.trace B w q)"
+  lemma dbcrai_snd[iff]: "infs (P \<circ> snd) (dra.trace (dbcrai A B) w (p, q)) \<longleftrightarrow> infs P (dca.trace B w q)"
   proof -
-    have "infs (P \<circ> snd) (dra.trace (dbcai A B) w (p, q)) \<longleftrightarrow>
-      infs P (smap snd (dra.trace (dbcai A B) w (p, q)))" by simp
-    also have "smap snd (dra.trace (dbcai A B) w (p, q)) = dca.trace B w q"
-      unfolding dbcai_def by (coinduction arbitrary: w p q) (auto)
+    let ?t = "dra.trace (dbcrai A B) w (p, q)"
+    have "infs (P \<circ> snd) ?t \<longleftrightarrow> infs P (smap snd ?t)" by simp
+    also have "smap snd ?t = dca.trace B w q" unfolding dbcrai_def by (coinduction arbitrary: w p q) (auto)
     finally show ?thesis by this
   qed
 
-  lemma dbcai_language: "DRA.language (dbcai A B) = DBA.language A \<inter> DCA.language B"
+  lemma dbcrai_language: "DRA.language (dbcrai A B) = DBA.language A \<inter> DCA.language B"
   proof -
-    have 0: "dra.alphabet (dbcai A B) = dba.alphabet A \<inter> dca.alphabet B" unfolding dbcai_def by simp
-    have 1: "dra.initial (dbcai A B) = (dba.initial A, dca.initial B)" unfolding dbcai_def by simp
-    have 2: "dra.accepting (dbcai A B) = [(dba.accepting A \<circ> fst, dca.rejecting B \<circ> snd)]"
-      unfolding dbcai_def by simp
-    have 3: "cogen rabin (dra.accepting (dbcai A B)) (DRA.trace (dbcai A B) w (p, q)) \<longleftrightarrow>
+    have 1: "dra.alphabet (dbcrai A B) = dba.alphabet A \<inter> dca.alphabet B" unfolding dbcrai_def by simp
+    have 2: "dra.initial (dbcrai A B) = (dba.initial A, dca.initial B)" unfolding dbcrai_def by simp
+    have 3: "dra.accepting (dbcrai A B) = [(dba.accepting A \<circ> fst, dca.rejecting B \<circ> snd)]"
+      unfolding dbcrai_def by simp
+    have 4: "cogen rabin (dra.accepting (dbcrai A B)) (DRA.trace (dbcrai A B) w (p, q)) \<longleftrightarrow>
       infs (dba.accepting A) (DBA.trace A w p) \<and> fins (rejecting B) (DCA.trace B w q)" for w p q
-      unfolding cogen_def rabin_def 2 by simp
+      unfolding cogen_def rabin_def 3 by simp
     show ?thesis
       unfolding DRA.language_def DBA.language_def DCA.language_def
       unfolding DRA.run_alt_def DBA.run_alt_def DCA.run_alt_def
-      unfolding 0 1 3 by auto
+      unfolding 1 2 4 by auto
   qed
 
   abbreviation (input) "get k pp \<equiv> pp ! k"
 
-  definition drau :: "('label, 'state) dra list \<Rightarrow> ('label, 'state list) dra" where
-    "drau AA \<equiv> dra
+  definition draul :: "('label, 'state) dra list \<Rightarrow> ('label, 'state list) dra" where
+    "draul AA \<equiv> dra
       (UNION (set AA) dra.alphabet)
       (map dra.initial AA)
       (\<lambda> a pp. map2 (\<lambda> A p. dra.succ A a p) AA pp)
       (do { k \<leftarrow> [0 ..< length AA]; (f, g) \<leftarrow> dra.accepting (AA ! k); [(f \<circ> get k, g \<circ> get k)] })"
 
-  lemma drau_trace:
+  lemma draul_get:
     assumes "length pp = length AA" "k < length AA"
-    shows "infs (P \<circ> get k) (dra.trace (drau AA) w pp) \<longleftrightarrow>
+    shows "infs (P \<circ> get k) (dra.trace (draul AA) w pp) \<longleftrightarrow>
       infs P (dra.trace (AA ! k) w (pp ! k))"
   proof -
-    have "infs (P \<circ> get k) (dra.trace (drau AA) w pp) \<longleftrightarrow>
-      infs P (smap (get k) (dra.trace (drau AA) w pp))" by simp
-    also have "smap (get k) (dra.trace (drau AA) w pp) = dra.trace (AA ! k) w (pp ! k)"
-      using assms unfolding drau_def by (coinduction arbitrary: w pp) (force)
+    have "infs (P \<circ> get k) (dra.trace (draul AA) w pp) \<longleftrightarrow>
+      infs P (smap (get k) (dra.trace (draul AA) w pp))" by simp
+    also have "smap (get k) (dra.trace (draul AA) w pp) = dra.trace (AA ! k) w (pp ! k)"
+      using assms unfolding draul_def by (coinduction arbitrary: w pp) (force)
     finally show ?thesis by this
   qed
 
-  lemma drau_language:
+  lemma draul_language:
     assumes "INTER (set AA) dra.alphabet = UNION (set AA) dra.alphabet"
-    shows "DRA.language (drau AA) = UNION (set AA) DRA.language"
+    shows "DRA.language (draul AA) = UNION (set AA) DRA.language"
   proof safe
     fix w
-    assume 1: "w \<in> DRA.language (drau AA)"
+    assume 1: "w \<in> DRA.language (draul AA)"
     obtain 2:
-      "dra.run (drau AA) w (dra.initial (drau AA))"
-      "cogen rabin (dra.accepting (drau AA)) (dra.trace (drau AA) w (dra.initial (drau AA)))"
+      "dra.run (draul AA) w (dra.initial (draul AA))"
+      "cogen rabin (dra.accepting (draul AA)) (dra.trace (draul AA) w (dra.initial (draul AA)))"
       using 1 by rule
     obtain I F where 3:
-      "(I, F) \<in> set (dra.accepting (drau AA))"
-      "infs I (dra.trace (drau AA) w (dra.initial (drau AA)))"
-      "fins F (dra.trace (drau AA) w (dra.initial (drau AA)))"
+      "(I, F) \<in> set (dra.accepting (draul AA))"
+      "infs I (dra.trace (draul AA) w (dra.initial (draul AA)))"
+      "fins F (dra.trace (draul AA) w (dra.initial (draul AA)))"
       using 2(2) by blast
     obtain k P Q where 4:
       "k < length AA" "I = P \<circ> get k" "F = Q \<circ> get k" "(P, Q) \<in> set (dra.accepting (AA ! k))"
-      using 3(1) unfolding drau_def List.bind_def by (auto simp: comp_def)
+      using 3(1) unfolding draul_def List.bind_def by (auto simp: comp_def)
     show "w \<in> UNION (set AA) DRA.language"
     proof (intro UN_I DRA.language cogen rabin)
       show "AA ! k \<in> set AA" using 4(1) by auto
       show "DRA.run (AA ! k) w (dra.initial (AA ! k))"
-        using assms 2(1) 4(1) unfolding DRA.run_alt_def drau_def by force
+        using assms 2(1) 4(1) unfolding DRA.run_alt_def draul_def by force
       show "(P, Q) \<in> set (dra.accepting (AA ! k))" using 4(4) by this
       show "(P, Q) = (P, Q)" by rule
-      have "True \<longleftrightarrow> infs (P \<circ> get k) (dra.trace (drau AA) w (map dra.initial AA))"
-        using 3(2) unfolding drau_def 4(2) by simp
+      have "True \<longleftrightarrow> infs (P \<circ> get k) (dra.trace (draul AA) w (map dra.initial AA))"
+        using 3(2) unfolding draul_def 4(2) by simp
       also have "\<dots> \<longleftrightarrow> infs P (dra.trace (AA ! k) w (map dra.initial AA ! k))"
-        using 4(1) by (force intro!: drau_trace)
+        using 4(1) by (force intro!: draul_get)
       also have "map dra.initial AA ! k = dra.initial (AA ! k)" using 4(1) by simp
       finally show "infs P (dra.trace (AA ! k) w (dra.initial (AA ! k)))" by simp
-      have "False \<longleftrightarrow> infs (Q \<circ> get k) (dra.trace (drau AA) w (map dra.initial AA))"
-        using 3(3) unfolding drau_def 4(3) by simp
+      have "False \<longleftrightarrow> infs (Q \<circ> get k) (dra.trace (draul AA) w (map dra.initial AA))"
+        using 3(3) unfolding draul_def 4(3) by simp
       also have "\<dots> \<longleftrightarrow> infs Q (dra.trace (AA ! k) w (map dra.initial AA ! k))"
-        using 4(1) by (force intro!: drau_trace)
+        using 4(1) by (force intro!: draul_get)
       also have "map dra.initial AA ! k = dra.initial (AA ! k)" using 4(1) by simp
       finally show "fins Q (dra.trace (AA ! k) w (dra.initial (AA ! k)))" by simp
     qed
@@ -127,27 +125,27 @@ begin
       "fins F (dra.trace A w (dra.initial A))"
       using 2(2) by blast
     obtain k where 4: "A = AA ! k" "k < length AA" using 1(1) unfolding in_set_conv_nth by auto
-    show "w \<in> DRA.language (drau AA)"
+    show "w \<in> DRA.language (draul AA)"
     proof (intro DRA.language cogen rabin)
-      show "dra.run (drau AA) w (dra.initial (drau AA))"
-        using 1(1) 2(1) unfolding DRA.run_alt_def drau_def by auto
-      show "(I \<circ> get k, F \<circ> get k) \<in> set (dra.accepting (drau AA))"
-        unfolding drau_def List.bind_def using 3(1) 4 by (force simp: comp_def)
+      show "dra.run (draul AA) w (dra.initial (draul AA))"
+        using 1(1) 2(1) unfolding DRA.run_alt_def draul_def by auto
+      show "(I \<circ> get k, F \<circ> get k) \<in> set (dra.accepting (draul AA))"
+        unfolding draul_def List.bind_def using 3(1) 4 by (force simp: comp_def)
       show "(I \<circ> get k, F \<circ> get k) = (I \<circ> get k, F \<circ> get k)" by rule
-      have "infs (I \<circ> get k) (dra.trace (drau AA) w (dra.initial (drau AA))) \<longleftrightarrow>
-        infs (I \<circ> get k) (dra.trace (drau AA) w (map dra.initial AA))"
-        unfolding drau_def by simp
+      have "infs (I \<circ> get k) (dra.trace (draul AA) w (dra.initial (draul AA))) \<longleftrightarrow>
+        infs (I \<circ> get k) (dra.trace (draul AA) w (map dra.initial AA))"
+        unfolding draul_def by simp
       also have "\<dots> \<longleftrightarrow> infs I (dra.trace (AA ! k) w (map dra.initial AA ! k))"
-        using 4(2) by (force intro!: drau_trace)
+        using 4(2) by (force intro!: draul_get)
       also have "\<dots> \<longleftrightarrow> True" using 3(2) 4 by simp
-      finally show "infs (I \<circ> get k) (dra.trace (drau AA) w (dra.initial (drau AA)))" by simp
-      have "infs (F \<circ> get k) (dra.trace (drau AA) w (dra.initial (drau AA))) \<longleftrightarrow>
-        infs (F \<circ> get k) (dra.trace (drau AA) w (map dra.initial AA))"
-        unfolding drau_def by simp
+      finally show "infs (I \<circ> get k) (dra.trace (draul AA) w (dra.initial (draul AA)))" by simp
+      have "infs (F \<circ> get k) (dra.trace (draul AA) w (dra.initial (draul AA))) \<longleftrightarrow>
+        infs (F \<circ> get k) (dra.trace (draul AA) w (map dra.initial AA))"
+        unfolding draul_def by simp
       also have "\<dots> \<longleftrightarrow> infs F (dra.trace (AA ! k) w (map dra.initial AA ! k))"
-        using 4(2) by (force intro!: drau_trace)
+        using 4(2) by (force intro!: draul_get)
       also have "\<dots> \<longleftrightarrow> False" using 3(3) 4 by simp
-      finally show "fins (F \<circ> get k) (dra.trace (drau AA) w (dra.initial (drau AA)))" by simp
+      finally show "fins (F \<circ> get k) (dra.trace (draul AA) w (dra.initial (draul AA)))" by simp
     qed
   qed
 
